restructatization

code/experimental/P256/Hacl.Impl.ECDSA.MM.Exponent.fst
@@ -33,14 +33,12 @@ val cswap: bit:uint64{v bit <= 1} -> p:felem -> q:felem
       modifies (loc p |+| loc q) h0 h1 /\
 	(
 	  let (r0, r1) = Hacl.Spec.ECDSA.conditional_swap bit (as_nat h0 p) (as_nat h0 q) in 
+	  let pBefore = as_seq h0 p in let qBefore = as_seq h0 q in 
+	  let pAfter = as_seq h1 p in let qAfter = as_seq h1 q in 
 	  if uint_v bit = 0 then r0 == as_nat h0 p /\ r1 == as_nat h0 q else r0 == as_nat h0 q /\ r1 == as_nat h0 p) /\
 	  as_nat h1 p < prime /\ as_nat h1 q < prime /\
-	
-      (
-	let pBefore = as_seq h0 p in let qBefore = as_seq h0 q in 
-	let pAfter = as_seq h1 p in let qAfter = as_seq h1 q in 
       (v bit == 1 ==> as_seq h1 p == as_seq h0 q /\ as_seq h1 q == as_seq h0 p) /\
-      (v bit == 0 ==> as_seq h1 p == as_seq h0 p /\ as_seq h1 q == as_seq h0 q)))
+      (v bit == 0 ==> as_seq h1 p == as_seq h0 p /\ as_seq h1 q == as_seq h0 q))
 
 
 let cswap bit p1 p2 =
@@ -83,15 +81,9 @@ val montgomery_ladder_exponent_step0: a: felem -> b: felem -> Stack unit
 let montgomery_ladder_exponent_step0 a b = 
     let h0 = ST.get() in 
   montgomery_multiplication_ecdsa_module a b b;
-    let h1 = ST.get() in 
-    assert(as_nat h1 b = toDomain_ (fromDomain_ (as_nat h0 a) * fromDomain_ (as_nat h0 b) % prime));
     lemmaToDomainFromDomain (fromDomain_ (as_nat h0 a) * fromDomain_ (as_nat h0 b) % prime);
-    assert(fromDomain_ (as_nat h1 b) = (fromDomain_ (as_nat h0 a) * fromDomain_ (as_nat h0 b) % prime));
   montgomery_multiplication_ecdsa_module a a a ;
-    let h2 = ST.get() in 
-    assert(fromDomain_ (as_nat h2 a) = fromDomain_ (toDomain_ (fromDomain_ (as_nat h0 a) * fromDomain_ (as_nat h0 a) % prime)));
-    lemmaToDomainFromDomain (fromDomain_ (as_nat h0 a) * fromDomain_ (as_nat h0 a) % prime);
-    assert(fromDomain_ (as_nat h2 a) = fromDomain_ (as_nat h0 a) * fromDomain_ (as_nat h0 a) % prime) 
+    lemmaToDomainFromDomain (fromDomain_ (as_nat h0 a) * fromDomain_ (as_nat h0 a) % prime)
 
 
 (* this piece of code is taken from Hacl.Curve25519 *)
@@ -113,10 +105,7 @@ let scalar_bit #buf_type s n =
   to_u64 ((s.(n /. 8ul) >>. (n %. 8ul)) &. u8 1)
 
 
-#reset-options "--z3refresh --z3rlimit 300"
-
-
-inline_for_extraction noextract 
+inline_for_extraction noextract
 val montgomery_ladder_exponent_step: a: felem -> b: felem -> scalar: ilbuffer uint8 (size 32) ->   i:size_t{v i < 256} ->  Stack unit
   (requires fun h -> live h a  /\ live h b /\ live h scalar /\ as_nat h a < prime /\ as_nat h b < prime /\ disjoint a b)
   (ensures fun h0 _ h1 -> modifies (loc a |+| loc b) h0 h1  /\
@@ -136,34 +125,13 @@ let montgomery_ladder_exponent_step a b scalar i =
   cswap bit a b;
   montgomery_ladder_exponent_step0 a b;
   cswap bit a b;
-      let h3 = ST.get() in 
-   Hacl.Spec.ECDSA.lemma_swaped_steps (fromDomain_ (as_nat h0 a)) (fromDomain_ (as_nat h0 b)); 
-  
+  Hacl.Spec.ECDSA.lemma_swaped_steps (fromDomain_ (as_nat h0 a)) (fromDomain_ (as_nat h0 b)); 
   [@inline_let]
   let k: Lib.Sequence.lseq uint8 32 = as_seq h0 scalar in 
   let open Lib.RawIntTypes in 
   [@inline_let]
   let bit_ = ith_bit k (255 - (uint_v i)) in 
-  assert(uint_to_nat bit_ == uint_v bit);
-
-  assert(
-    let a_ = fromDomain_ (as_nat h0 a) in 
-    let b_ = fromDomain_ (as_nat h0 b) in 
-      if uint_v bit = 0 then 
-	let (r0D, r1D) = _exp_step0 a_ b_ in 
-	r0D == fromDomain_ (as_nat h3 a) /\ r1D == fromDomain_ (as_nat h3 b)
-      else
-	let (r0D, r1D) = _exp_step1 a_ b_ in 
-	r0D == fromDomain_ (as_nat h3 a) /\ r1D == fromDomain_ (as_nat h3 b)); 
-	
-   assert(
-     let a_ = fromDomain_ (as_nat h0 a) in 
-     let b_ = fromDomain_ (as_nat h0 b) in 
-     let (r0D, r1D) = _exp_step k (uint_v i) (a_, b_) in 
-     r0D == fromDomain_ (as_nat h3 a) /\ r1D == fromDomain_ (as_nat h3 b));
-
-   assert(modifies (loc a |+| loc b) h0 h3);
-   assert(as_nat h3 a < prime /\ as_nat h3 b < prime)
+  ()
 
 
 inline_for_extraction noextract 
@@ -182,16 +150,11 @@ val _montgomery_ladder_exponent: a: felem ->b: felem ->  scalar: ilbuffer uint8 
   
 let _montgomery_ladder_exponent a b scalar = 
   let h0 = ST.get() in 
-
   [@inline_let]
   let spec_exp h0  = _exp_step (as_seq h0 scalar) in 
-
   [@inline_let]
-  let acc (h: mem) : GTot (tuple2 nat_prime nat_prime) = 
-    (fromDomain_ (as_nat h a), fromDomain_ (as_nat h b)) in 
-
+  let acc (h: mem) : GTot (tuple2 nat_prime nat_prime) = (fromDomain_ (as_nat h a), fromDomain_ (as_nat h b)) in 
   Lib.LoopCombinators.eq_repeati0 256 (spec_exp h0) (acc h0);
-
   [@inline_let]
   let inv h (i: nat {i <= 256}) = 
     live h a /\ live h b /\ live h scalar /\ 
@@ -199,24 +162,10 @@ let _montgomery_ladder_exponent a b scalar =
     as_nat h a < prime /\ as_nat h b < prime /\
     acc h == Lib.LoopCombinators.repeati i (spec_exp h0) (acc h0)     
     in 
-
   for 0ul 256ul inv (
     fun i -> 
-	let h3 = ST.get() in
 	  montgomery_ladder_exponent_step a b scalar i;
-	  let h4 = ST.get() in   
-	  assert(modifies2 a b h3 h4);
-	  assert(modifies2 a b h0 h4);
-	  assert(
-	    let a_ = fromDomain_ (as_nat h3 a) in 
-	    let b_ = fromDomain_ (as_nat h3 b) in 
-	    let (r0D, r1D) = _exp_step (as_seq h0 scalar) (uint_v i) (a_, b_) in  
-	    r0D == fromDomain_ (as_nat h4 a));
-
-	  Lib.LoopCombinators.unfold_repeati 256 (spec_exp h0) (acc h0) (uint_v i);
-	assert(acc h4 == Lib.LoopCombinators.repeati (uint_v i + 1) (spec_exp h0) (acc h0))
-  )
-
+	  Lib.LoopCombinators.unfold_repeati 256 (spec_exp h0) (acc h0) (uint_v i))
 
 
 inline_for_extraction noextract 
@@ -245,22 +194,11 @@ let upload_one b =
 let montgomery_ladder_exponent r = 
   push_frame(); 
     let p = create (size 4) (u64 0) in 
-      let h0 = ST.get() in 
     upload_one_montg_form p; 
-      let h1 = ST.get() in 
     recall_contents order_inverse_buffer prime_p256_order_inverse_seq;
     _montgomery_ladder_exponent p r order_inverse_buffer;
-      let h2 = ST.get() in 
       lemmaToDomainFromDomain 1;
-      assert(
-	let b_ = fromDomain_ (as_nat h0 r) in 
-	let (r0D, r1D) = _exponent_spec prime_p256_order_inverse_seq (1, b_) in 
-	r0D == fromDomain_ (as_nat h2 p));     
-      assert(as_nat h2 p < prime);
     copy r p;
-      let h3 = ST.get() in 
-      assert(as_nat h3 r == as_nat h2 p);
-      assert(as_nat h3 r < prime);
   pop_frame()  
 
 
@@ -268,10 +206,7 @@ let fromDomainImpl a result =
   push_frame();
     let one = create (size 4) (u64 0) in 
     upload_one one;
-      let h1 = ST.get() in 
     montgomery_multiplication_ecdsa_module one a result;
-      let h2 = ST.get() in 
-      assert(as_nat h2 result = fromDomain_(as_nat h1 a));
   pop_frame()   
 
 
@@ -279,12 +214,9 @@ val lemma_fromDomain1: a: nat ->
   Lemma ((fromDomain_ (fromDomain_ (fromDomain_ a))) == ((a * modp_inv2_prime (pow2 256) prime_p256_order * modp_inv2_prime (pow2 256) prime_p256_order * modp_inv2_prime (pow2 256) prime_p256_order) % prime_p256_order))
 
 let lemma_fromDomain1 a = 
-  let a_ = fromDomain_ (fromDomain_ (fromDomain_ a)) in 
   let f = modp_inv2_prime (pow2 256) prime_p256_order in 
   lemma_mod_mul_distr_l (a * f) f prime_p256_order; 
-  lemma_mod_mul_distr_l (a * f * f) f prime_p256_order;
-  
-  assert(a_ == ((a * modp_inv2_prime (pow2 256) prime_p256_order * modp_inv2_prime (pow2 256) prime_p256_order * modp_inv2_prime (pow2 256) prime_p256_order) % prime_p256_order))
+  lemma_mod_mul_distr_l (a * f * f) f prime_p256_order
 
 (* fermat little theorem *)
 val lemma_l_ferm: a: nat -> Lemma (pow a (prime_p256_order - 1) % prime_p256_order == 1)
@@ -337,27 +269,15 @@ let multPower a b result =
       fromDomainImpl a tempB1;
       fromDomainImpl b buffFromDB;
       fromDomainImpl buffFromDB buffFromDB;
-	let h1 = ST.get() in 
-	assert(as_nat h1 tempB1 == fromDomain_ (as_nat h0 a));
-	assert(as_nat h1 buffFromDB == fromDomain_ (fromDomain_ (as_nat h0 b)));
       montgomery_ladder_exponent tempB1;
-	let h2 = ST.get() in 
-	assert(let r0D = exponent_spec (fromDomain_ (fromDomain_ (as_nat h0 a))) in fromDomain_ (as_nat h2 tempB1) == r0D);
       montgomery_multiplication_ecdsa_module tempB1 buffFromDB result;
-	let h3 = ST.get() in 
-
     pop_frame();
     
       let p = pow (fromDomain_ (fromDomain_ (as_nat h0 a))) (prime_p256_order - 2) % prime_p256_order in 
       let q = fromDomain_ (fromDomain_ (fromDomain_ (as_nat h0 b))) in 
-      assert(as_nat h3 result = toDomain_ ((p * q) % prime_p256_order));
       let r = modp_inv2_prime (pow2 256) prime_p256_order in 
       lemma_fromDomain1 (as_nat h0 b);
       lemma_fromDomain2 (as_nat h0 a);
-
-	assert(p == (pow (as_nat h0 a) (prime_p256_order - 2) * pow r (prime_p256_order - 2) * pow r (prime_p256_order - 2)) % prime_p256_order); 
-	assert(q ==  (((as_nat h0 b) * r * r * r) % prime_p256_order));
-
     let open FStar.Tactics in 
     let open FStar.Tactics.Canon in 
 
@@ -369,95 +289,51 @@ let multPower a b result =
       power_one r;
       assert(pow r 1 == r);
       assert(pow r (prime_p256_order -2) * r == pow r (prime_p256_order - 1));
-      
-      assert(as_nat h3 result = toDomain_ ((pow (as_nat h0 a) (prime_p256_order - 2) * (pow r (prime_p256_order - 2) * r) * (pow r (prime_p256_order - 2) * r) * (as_nat h0 b) * r) % prime_p256_order));
-      assert(pow (as_nat h0 a) (prime_p256_order - 2) * (pow r (prime_p256_order - 2) * r) * (pow r (prime_p256_order - 2) * r) * (as_nat h0 b) * r == pow (as_nat h0 a) (prime_p256_order - 2) * (pow r (prime_p256_order - 1)) * (pow r (prime_p256_order - 1)) * (as_nat h0 b) * r);
-       lemma_mod_mul_distr_l (pow (as_nat h0 a) (prime_p256_order - 2) * (pow r (prime_p256_order - 1)) * (pow r (prime_p256_order - 1)) * (as_nat h0 b) * r) (pow2 256) prime_p256_order;
+      lemma_mod_mul_distr_l (pow (as_nat h0 a) (prime_p256_order - 2) * (pow r (prime_p256_order - 1)) * (pow r (prime_p256_order - 1)) * (as_nat h0 b) * r) (pow2 256) prime_p256_order;
 
       assert_by_tactic (pow (as_nat h0 a) (prime_p256_order - 2) * (pow r (prime_p256_order - 1)) * (pow r (prime_p256_order - 1)) * (as_nat h0 b) * r * pow2 256 == pow (as_nat h0 a) (prime_p256_order - 2) * (pow r (prime_p256_order - 1)) * (pow r (prime_p256_order - 1)) * (as_nat h0 b) * (r * pow2 256)) canon;
       lemma_mod_mul_distr_r (pow (as_nat h0 a) (prime_p256_order - 2) * (pow r (prime_p256_order - 1)) * (pow r (prime_p256_order - 1)) * (as_nat h0 b)) (r * pow2 256) prime_p256_order;
       assert_norm ((pow2 256 * modp_inv2_prime (pow2 256) prime_p256_order) % prime_p256_order == 1);
-      assert(as_nat h3 result = (pow (as_nat h0 a) (prime_p256_order - 2) * (pow r (prime_p256_order - 1)) * (pow r (prime_p256_order - 1)) * (as_nat h0 b)) % prime_p256_order);
-
       assert_by_tactic (pow (as_nat h0 a) (prime_p256_order - 2) * (pow r (prime_p256_order - 1)) * (pow r (prime_p256_order - 1)) * (as_nat h0 b) == pow (as_nat h0 a) (prime_p256_order - 2) * (as_nat h0 b)  * (pow r (prime_p256_order - 1)) * (pow r (prime_p256_order - 1))) canon;
-
-    
       lemma_mod_mul_distr_r (pow (as_nat h0 a) (prime_p256_order - 2) * (as_nat h0 b)  * (pow r (prime_p256_order - 1))) (pow r (prime_p256_order - 1)) prime_p256_order;
       lemma_l_ferm r;
-      
-      assert(as_nat h3 result = (pow (as_nat h0 a) (prime_p256_order - 2)  * (as_nat h0 b) * (pow r (prime_p256_order - 1))) % prime_p256_order);
-      
       lemma_mod_mul_distr_r (pow (as_nat h0 a) (prime_p256_order - 2) * (as_nat h0 b)) (pow r (prime_p256_order - 1)) prime_p256_order;
-      lemma_l_ferm r;
+      lemma_l_ferm r
 
-      assert(as_nat h3 result = (pow (as_nat h0 a) (prime_p256_order - 2)  * (as_nat h0 b)) % prime_p256_order)
-
-(* 
-val multPowerPartial: s: felem -> a: felem -> b: felem -> result: felem -> Stack unit 
-  (requires fun h -> live h a /\ live h b /\ live h result /\ as_nat h a < prime /\ as_nat h b < prime /\ 
-  (
-      let a_ = fromDomain_  (fromDomain_ (as_nat h s)) in 
-      let r0D = exponent_spec a_ in 
-      fromDomain_ (as_nat h a) == r0D)
-  )
-  (ensures fun h0 _ h1 -> modifies (loc result) h0 h1)
-*)
 
 let multPowerPartial s a b result = 
   let h0 = ST.get() in 
       assert(let r0D = exponent_spec (fromDomain_  (fromDomain_ (as_nat h0 s))) in fromDomain_ (as_nat h0 a) == r0D);
   push_frame();
     let buffFromDB = create (size 4) (u64 0) in 
-      let h1 = ST.get() in 
     fromDomainImpl b buffFromDB;
     fromDomainImpl buffFromDB buffFromDB;
-      let h2 = ST.get() in 
     montgomery_multiplication_ecdsa_module a buffFromDB result;
-      let h3 = ST.get() in 
   pop_frame();
-    assert(as_nat h2 buffFromDB == fromDomain_ (fromDomain_ (as_nat h0 b)));
 
     let p = pow (fromDomain_ (fromDomain_ (as_nat h0 s))) (prime_p256_order - 2) % prime_p256_order in 
     let q = fromDomain_ (fromDomain_ (fromDomain_ (as_nat h0 b))) in 
-    assert(as_nat h3 result = toDomain_ ((p * q) % prime_p256_order));
     let r = modp_inv2_prime (pow2 256) prime_p256_order in 
       lemma_fromDomain1 (as_nat h0 b);
       lemma_fromDomain2 (as_nat h0 s);
-
-      assert(p == (pow (as_nat h0 s) (prime_p256_order - 2) * pow r (prime_p256_order - 2) * pow r (prime_p256_order - 2)) % prime_p256_order); 
-      assert(q ==  (((as_nat h0 b) * r * r * r) % prime_p256_order));
 
     let open FStar.Tactics in 
     let open FStar.Tactics.Canon in 
 
     lemma_mod_mul_distr_l (pow (as_nat h0 s) (prime_p256_order - 2) * pow r (prime_p256_order - 2) * pow r (prime_p256_order - 2)) (((as_nat h0 b) * r * r * r) % prime_p256_order) prime_p256_order;
     lemma_mod_mul_distr_r (pow (as_nat h0 s) (prime_p256_order - 2) * pow r (prime_p256_order - 2) * pow r (prime_p256_order - 2)) ((as_nat h0 b) * r * r * r) prime_p256_order;
-
       assert_by_tactic (pow (as_nat h0 s) (prime_p256_order - 2) * pow r (prime_p256_order - 2) * pow r (prime_p256_order - 2) * ((as_nat h0 b) * r * r * r) == pow (as_nat h0 s) (prime_p256_order - 2) * (pow r (prime_p256_order - 2) * r) * (pow r (prime_p256_order - 2) * r) * (as_nat h0 b) * r) canon;
       pow_plus r (prime_p256_order - 2) 1; 
       power_one r;
       assert(pow r 1 == r);
       assert(pow r (prime_p256_order -2) * r == pow r (prime_p256_order - 1));
-
-      assert(as_nat h3 result = toDomain_ ((pow (as_nat h0 s) (prime_p256_order - 2) * (pow r (prime_p256_order - 2) * r) * (pow r (prime_p256_order - 2) * r) * (as_nat h0 b) * r) % prime_p256_order));
-      assert(pow (as_nat h0 s) (prime_p256_order - 2) * (pow r (prime_p256_order - 2) * r) * (pow r (prime_p256_order - 2) * r) * (as_nat h0 b) * r == pow (as_nat h0 s) (prime_p256_order - 2) * (pow r (prime_p256_order - 1)) * (pow r (prime_p256_order - 1)) * (as_nat h0 b) * r);
-       lemma_mod_mul_distr_l (pow (as_nat h0 s) (prime_p256_order - 2) * (pow r (prime_p256_order - 1)) * (pow r (prime_p256_order - 1)) * (as_nat h0 b) * r) (pow2 256) prime_p256_order;
-
+      lemma_mod_mul_distr_l (pow (as_nat h0 s) (prime_p256_order - 2) * (pow r (prime_p256_order - 1)) * (pow r (prime_p256_order - 1)) * (as_nat h0 b) * r) (pow2 256) prime_p256_order;
       assert_by_tactic (pow (as_nat h0 s) (prime_p256_order - 2) * (pow r (prime_p256_order - 1)) * (pow r (prime_p256_order - 1)) * (as_nat h0 b) * r * pow2 256 == pow (as_nat h0 s) (prime_p256_order - 2) * (pow r (prime_p256_order - 1)) * (pow r (prime_p256_order - 1)) * (as_nat h0 b) * (r * pow2 256)) canon;
       lemma_mod_mul_distr_r (pow (as_nat h0 s) (prime_p256_order - 2) * (pow r (prime_p256_order - 1)) * (pow r (prime_p256_order - 1)) * (as_nat h0 b)) (r * pow2 256) prime_p256_order;
       assert_norm ((pow2 256 * modp_inv2_prime (pow2 256) prime_p256_order) % prime_p256_order == 1);
-      assert(as_nat h3 result = (pow (as_nat h0 s) (prime_p256_order - 2) * (pow r (prime_p256_order - 1)) * (pow r (prime_p256_order - 1)) * (as_nat h0 b)) % prime_p256_order);
-
       assert_by_tactic (pow (as_nat h0 s) (prime_p256_order - 2) * (pow r (prime_p256_order - 1)) * (pow r (prime_p256_order - 1)) * (as_nat h0 b) == pow (as_nat h0 s) (prime_p256_order - 2) * (as_nat h0 b)  * (pow r (prime_p256_order - 1)) * (pow r (prime_p256_order - 1))) canon;
-
-    
       lemma_mod_mul_distr_r (pow (as_nat h0 s) (prime_p256_order - 2) * (as_nat h0 b)  * (pow r (prime_p256_order - 1))) (pow r (prime_p256_order - 1)) prime_p256_order;
       lemma_l_ferm r;
-      
-      assert(as_nat h3 result = (pow (as_nat h0 s) (prime_p256_order - 2)  * (as_nat h0 b) * (pow r (prime_p256_order - 1))) % prime_p256_order);
-      
       lemma_mod_mul_distr_r (pow (as_nat h0 s) (prime_p256_order - 2) * (as_nat h0 b)) (pow r (prime_p256_order - 1)) prime_p256_order;
-      lemma_l_ferm r;
-
-      assert(as_nat h3 result = (pow (as_nat h0 s) (prime_p256_order - 2)  * (as_nat h0 b)) % prime_p256_order)
+      lemma_l_ferm r
 
