code/experimental/P256/Hacl.Impl.LowLevel.fst
@@ -10,6 +10,7 @@ open Lib.Buffer
 open Hacl.Spec.P256.Definitions
 open Hacl.Spec.P256.Lemmas
 open Hacl.Spec.P256.Basic
+open Hacl.Spec.ECDSA
 
 open FStar.Math.Lemmas
 open FStar.Mul
@@ -317,3 +318,22 @@ let shift8 t out =
   upd out (size 5) t6;
   upd out (size 6) t7;
   upd out (size 7) (u64 0)
+
+(* this piece of code is taken from Hacl.Curve25519 *)
+inline_for_extraction noextract
+val scalar_bit:
+    #buf_type: buftype -> 
+    s:lbuffer_t buf_type uint8 (size 32)
+  -> n:size_t{v n < 256}
+  -> Stack uint64
+    (requires fun h0 -> live h0 s)
+    (ensures  fun h0 r h1 -> h0 == h1 /\
+      r == ith_bit (as_seq h0 s) (v n) /\ v r <= 1)
+      
+let scalar_bit #buf_type s n =
+  let h0 = ST.get () in
+  mod_mask_lemma ((Lib.Sequence.index (as_seq h0 s) (v n / 8)) >>. (n %. 8ul)) 1ul;
+  assert_norm (1 = pow2 1 - 1);
+  assert (v (mod_mask #U8 #SEC 1ul) == v (u8 1));
+  to_u64 ((s.(n /. 8ul) >>. (n %. 8ul)) &. u8 1)
+
